Address PR comments
Move Client's use of MessageBody.Encrypt to a local method in Client.dfy.
Move const declarations earlier in file.
Add START_SEQUENCE_NUMBER const.
Break EncryptFrame into EncryptRegularFrame and EncryptFinalFrame.

src/SDK/MessageBody.dfy
@@ -6,7 +6,7 @@ include "../Crypto/AESEncryption.dfy"
 
 module MessageBody {
   export
-    provides EncryptMessageBody, Encrypt
+    provides EncryptMessageBody
     provides StandardLibrary, UInt, Msg, AlgorithmSuite
 
   import opened StandardLibrary
@@ -15,52 +15,52 @@ module MessageBody {
   import Msg = MessageHeader
   import AESEncryption
 
+  const BODY_AAD_CONTENT_REGULAR_FRAME := StringToByteSeq("AWSKMSEncryptionClient Frame");
+  const BODY_AAD_CONTENT_FINAL_FRAME := StringToByteSeq("AWSKMSEncryptionClient Final Frame");
+
+  const START_SEQUENCE_NUMBER: uint32 := 1
+  const ENDFRAME_SEQUENCE_NUMBER: uint32 := 0xFFFF_FFFF
+
   method EncryptMessageBody(plaintext: seq<uint8>, frameLength: int, messageID: Msg.MessageID, key: seq<uint8>, algorithmSuiteID: AlgorithmSuite.ID) returns (res: Result<seq<uint8>>)
     requires |key| == algorithmSuiteID.KeyLength()
     requires 0 < frameLength < UINT32_LIMIT
   {
     var body := [];
-    var n, sequenceNumber := 0, 1;
+    var n, sequenceNumber := 0, START_SEQUENCE_NUMBER;
     while n + frameLength <= |plaintext|
       invariant 0 <= n <= |plaintext|
-      invariant sequenceNumber <= ENDFRAME_SEQUENCE_NUMBER
+      invariant START_SEQUENCE_NUMBER <= sequenceNumber <= ENDFRAME_SEQUENCE_NUMBER
     {
       if sequenceNumber == ENDFRAME_SEQUENCE_NUMBER {
         return Failure("too many frames");
       }
       var plaintextFrame := plaintext[n..n + frameLength];
-      var regularFrame :- EncryptFrame(algorithmSuiteID, key, frameLength, messageID, plaintextFrame, sequenceNumber, false);
+      var regularFrame :- EncryptRegularFrame(algorithmSuiteID, key, frameLength, messageID, plaintextFrame, sequenceNumber);
       body := body + regularFrame;
       n, sequenceNumber := n + frameLength, sequenceNumber + 1;
     }
-    var finalFrame :- EncryptFrame(algorithmSuiteID, key, frameLength, messageID, plaintext[n..], sequenceNumber, true);
+    var finalFrame :- EncryptFinalFrame(algorithmSuiteID, key, frameLength, messageID, plaintext[n..], sequenceNumber);
     body := body + finalFrame;
     return Success(body);
   }
 
-  method EncryptFrame(algorithmSuiteID: AlgorithmSuite.ID, key: seq<uint8>, frameLength: int, messageID: Msg.MessageID,
-                      plaintext: seq<uint8>, sequenceNumber: uint32, final: bool)
+  method EncryptRegularFrame(algorithmSuiteID: AlgorithmSuite.ID, key: seq<uint8>, frameLength: int,
+                             messageID: Msg.MessageID, plaintext: seq<uint8>, sequenceNumber: uint32)
       returns (res: Result<seq<uint8>>)
     requires |key| == algorithmSuiteID.KeyLength()
-    requires 0 < frameLength && 0 < sequenceNumber <= ENDFRAME_SEQUENCE_NUMBER
+    requires 0 < frameLength && START_SEQUENCE_NUMBER <= sequenceNumber <= ENDFRAME_SEQUENCE_NUMBER
     requires |plaintext| < UINT32_LIMIT
-    requires !final ==> |plaintext| == frameLength && sequenceNumber != ENDFRAME_SEQUENCE_NUMBER
-    requires final ==> |plaintext| < frameLength
+    requires |plaintext| == frameLength && sequenceNumber != ENDFRAME_SEQUENCE_NUMBER
     requires 4 <= algorithmSuiteID.IVLength()
   {
-    var unauthenticatedFrame := if final then UInt32ToSeq(ENDFRAME_SEQUENCE_NUMBER) else [];
     var seqNumSeq := UInt32ToSeq(sequenceNumber as uint32);
-    unauthenticatedFrame := unauthenticatedFrame + seqNumSeq;
+    var unauthenticatedFrame := seqNumSeq;
 
     var iv: seq<uint8> := seq(algorithmSuiteID.IVLength() - 4, _ => 0) + UInt32ToSeq(sequenceNumber as uint32);
     assert |iv| == algorithmSuiteID.IVLength();
     unauthenticatedFrame := unauthenticatedFrame + iv;
 
-    if final {
-      unauthenticatedFrame := unauthenticatedFrame + UInt32ToSeq(|plaintext| as uint32);
-    }
-
-    var contentAAD := if final then BODY_AAD_CONTENT_FINAL_FRAME else BODY_AAD_CONTENT_REGULAR_FRAME;
+    var contentAAD := BODY_AAD_CONTENT_REGULAR_FRAME;
     var aad := messageID + contentAAD + seqNumSeq + UInt64ToSeq(|plaintext| as uint64);
 
     var pair :- Encrypt(algorithmSuiteID, iv, key, plaintext, aad);
@@ -70,10 +70,34 @@ module MessageBody {
     return Success(unauthenticatedFrame);
   }
 
-  const BODY_AAD_CONTENT_REGULAR_FRAME := StringToByteSeq("AWSKMSEncryptionClient Frame");
-  const BODY_AAD_CONTENT_FINAL_FRAME := StringToByteSeq("AWSKMSEncryptionClient Final Frame");
+  method EncryptFinalFrame(algorithmSuiteID: AlgorithmSuite.ID, key: seq<uint8>, frameLength: int,
+                           messageID: Msg.MessageID, plaintext: seq<uint8>, sequenceNumber: uint32)
+      returns (res: Result<seq<uint8>>)
+    requires |key| == algorithmSuiteID.KeyLength()
+    requires 0 < frameLength && START_SEQUENCE_NUMBER <= sequenceNumber <= ENDFRAME_SEQUENCE_NUMBER
+    requires |plaintext| < UINT32_LIMIT
+    requires |plaintext| < frameLength
+    requires 4 <= algorithmSuiteID.IVLength()
+  {
+    var unauthenticatedFrame := UInt32ToSeq(ENDFRAME_SEQUENCE_NUMBER);
+    var seqNumSeq := UInt32ToSeq(sequenceNumber as uint32);
+    unauthenticatedFrame := unauthenticatedFrame + seqNumSeq;
 
-  const ENDFRAME_SEQUENCE_NUMBER: uint32 := 0xFFFF_FFFF
+    var iv: seq<uint8> := seq(algorithmSuiteID.IVLength() - 4, _ => 0) + UInt32ToSeq(sequenceNumber as uint32);
+    assert |iv| == algorithmSuiteID.IVLength();
+    unauthenticatedFrame := unauthenticatedFrame + iv;
+
+    unauthenticatedFrame := unauthenticatedFrame + UInt32ToSeq(|plaintext| as uint32);
+
+    var contentAAD := BODY_AAD_CONTENT_FINAL_FRAME;
+    var aad := messageID + contentAAD + seqNumSeq + UInt64ToSeq(|plaintext| as uint64);
+
+    var pair :- Encrypt(algorithmSuiteID, iv, key, plaintext, aad);
+    var (encryptedContents, authTag) := pair;
+    unauthenticatedFrame := unauthenticatedFrame + encryptedContents + authTag;
+
+    return Success(unauthenticatedFrame);
+  }
 
   method Encrypt(algorithmSuiteID: AlgorithmSuite.ID, iv: seq<uint8>, key: seq<uint8>, plaintext: seq<uint8>, aad: seq<uint8>) returns (res: Result<(seq<uint8>,seq<uint8>)>)
     requires |iv| == algorithmSuiteID.IVLength()
